src/drf/PF.v
@@ -1,14 +1,14 @@
 Require Import Omega.
 Require Import RelationClasses.
 
-Require Import sflib.
+From sflib Require Import sflib.
 
-Require Import Axioms.
-Require Import Basic.
-Require Import DataStructure.
+From PromisingLib Require Import Axioms.
+From PromisingLib Require Import Basic.
+From PromisingLib Require Import DataStructure.
 Require Import Time.
 Require Import Event.
-Require Import Language.
+From PromisingLib Require Import Language.
 Require Import View.
 Require Import Cell.
 Require Import Memory.
@@ -21,13 +21,13 @@ Require Import Progress.
 
 Set Implicit Arguments.
 
-Inductive pftstep: forall (e:option Event.t) (tid:Ident.t) (c1 c2: Configuration.t), Prop :=
+Inductive pftstep: forall (e:MachineEvent.t) (tid:Ident.t) (c1 c2: Configuration.t), Prop :=
 | pftstep_intro
     e tid c1 lang st1 lc1 e2 st3 lc3 sc3 memory3
     (TID: IdentMap.find tid c1.(Configuration.threads) = Some (existT _ lang st1, lc1))
     (STEPS: rtc (tau (@Thread.program_step _)) (Thread.mk _ st1 lc1 c1.(Configuration.sc) c1.(Configuration.memory)) e2)
     (STEP: Thread.program_step e e2 (Thread.mk _ st3 lc3 sc3 memory3)):
-    pftstep (ThreadEvent.get_event e) tid c1 (Configuration.mk (IdentMap.add tid (existT _ _ st3, lc3) c1.(Configuration.threads)) sc3 memory3)
+    pftstep (ThreadEvent.get_machine_event e) tid c1 (Configuration.mk (IdentMap.add tid (existT _ _ st3, lc3) c1.(Configuration.threads)) sc3 memory3)
 .
 Hint Constructors pftstep.
 
@@ -35,13 +35,13 @@ Definition pftstep_all (c0 c1: Configuration.t) :=
   union (fun e => union (pftstep e)) c0 c1.
 Hint Unfold pftstep_all.
 
-Inductive opt_pftstep lang : option Event.t -> Thread.t lang -> Thread.t lang -> Prop :=
-| opt_pftstep_none
-    c:
-    opt_pftstep None c c
-| opt_pftstep_some
-    e e1 e2
-    (STEP: Thread.program_step e e1 e2):
-    opt_pftstep (ThreadEvent.get_event e) e1 e2
+Inductive opt_pftstep: forall (e: MachineEvent.t) (tid: Ident.t) (c1 c2: Configuration.t), Prop :=
+| pftstep_none
+    tid c:
+    opt_pftstep MachineEvent.silent tid c c
+| pftstep_some
+    e tid c1 c2
+    (STEP: pftstep e tid c1 c2):
+    opt_pftstep e tid c1 c2
 .
 Hint Constructors opt_pftstep.
